\usepackage{mathtools}

\begin{itemize}
    \item $\sum_{k=0}^{n} k^2 = n(n+1)(2n+1)/6$
    \item $\sum_{k=0}^{n} k^3 = n^2(n+1)^2/4$
    \item $\sum_{k=0}^{n} k^4 = (6n^5+15n^4+10n^3-n)/30$
    \item $\sum_{k=0}^{n} k^5 = (2n^6+6n^5+5n^4-n^2)/12$
    \item $\sum_{k=0}^{n} kx^{k} = (x - (n+1)x^{n+1} + nx^{n+2}) / (x-1)^2$
    \item $(n+1)^{k+1} - 1 = \sum_{m=1}^{n} ((m+1)^{k+1} - m^{k+1}) = \sum_{p=0}^{k} \binom{k+1}{p}(1^p + 2^p + ... + n^p)$
    \item $\sum_{k=0}^{n} k \binom{n}{k} = n2^{n-1}$
    \item $\sum_{k=0}^{n} k^2 \binom{n}{k} = (n + n^2)2^{n-2}$
    \item $\sum_{j=0}^{k} \binom{m}{j} \binom{n-m}{k-j} = \binom{n}{k}$
    \item $\sum_{m=0}^{n} \binom{m}{k} = \binom{n+1}{k+1}$
    \item $\sum_{j=0}^{m} \binom{m}{j}^2 = \binom{2m}{m}$
    \item $\sum_{k=0}^{\lfloor\frac{n}{2}\rfloor} \binom{n-k}{k} = F(n+1)$
    \item $\sum_{i=0}^{n} i \binom{n}{i}^2 = \frac{n}{2} \binom{2n}{n}$
    \item $\sum_{i=0}^{n} i^2 \binom{n}{i}^2 = n^2 \binom{2n-2}{n-1}$
    \item $\sum_{k=q}^{n} \binom{n}{k}\binom{k}{q} = 2^{n-q}\binom{n}{q}$
    \item $\sum_{k=-a}^{a} (-1)^k \binom{2a}{k+a}^3 = \frac{(3a)!}{(a!)^3}$
    \item $\sum_{k=-a}^{a} (-1)^k \binom{a+b}{a+k}\binom{b+c}{b+k}\binom{c+a}{c+k} = \frac{(a+b+c)!}{a!b!c!}$
\end{itemize}
